feat(core): more instances for Range, RangeTo, RangeFrom

proof-libs/fstar/core/Core.Ops.Range.fsti
@@ -35,45 +35,75 @@ instance iterator_range t: iterator (t_Range (Rust_primitives.int_t t)) =
 
 open Core.Ops.Index
 
-instance impl_range_index_slice t len n : t_Index (t_Array t len) (t_Range (int_t n)) = {
-  f_Output = t_Slice t;
-  in_range = (fun (arr: t_Array t len) {f_start; f_end} -> 
-    v f_start >= 0     /\
-    v f_start <= v len /\
-    v f_end   <= v len
-  );
-  f_index = (fun arr {f_start; f_end} -> 
-      if f_start <. f_end
-      then Seq.slice arr (v f_start) (v f_end)
-      else Seq.empty
-    );
-}
+instance impl_index_range_slice t n : t_Index (t_Slice t) (t_Range (int_t n)) 
+  = { f_Output = t_Slice t
+    ; in_range = (fun (s: t_Slice t) {f_start; f_end} -> 
+         let len = Rust_primitives.length s in
+         v f_start >= 0 /\ v f_start <= v len /\ v f_end <= v len)
+    ; f_index = (fun s {f_start; f_end} -> 
+          if f_start <. f_end then Seq.slice s (v f_start) (v f_end)
+                              else Seq.empty)}
 
-instance impl_index_range_array t n : t_Index (t_Slice t) (t_Range (int_t n)) = {
-  f_Output = t_Slice t;
-  in_range = (fun (s: t_Slice t) {f_start; f_end} -> 
-    let len = Rust_primitives.length s in
-    v f_start >= 0     /\
-    v f_start <= v len /\
-    v f_end   <= v len
-  );
-  f_index = (fun s {f_start; f_end} -> 
-      if f_start <. f_end
-      then Seq.slice s (v f_start) (v f_end)
-      else Seq.empty
-    );
-}
+instance impl_index_range_to_slice t n : t_Index (t_Slice t) (t_RangeTo (int_t n)) 
+  = { f_Output = t_Slice t
+    ; in_range = (fun (s: t_Slice t) ({f_end}: t_RangeTo (int_t n)) -> 
+         let len = Rust_primitives.length s in v f_end <= v len)
+    ; f_index = (fun s {f_end} -> if 0 < v f_end then Seq.slice s 0 (v f_end) else Seq.empty)}
+
+instance impl_index_range_from_slice t n : t_Index (t_Slice t) (t_RangeFrom (int_t n)) 
+  = { f_Output = t_Slice t
+    ; in_range = (fun (s: t_Slice t) ({f_start}: t_RangeFrom (int_t n)) -> 
+         let len = Rust_primitives.length s in v f_start >= 0 /\ v f_start <= v len)
+    ; f_index = (fun s {f_start} -> 
+         let len = Rust_primitives.length s in
+         if v f_start = v len then Seq.empty else Seq.slice s (v f_start) (v len))}
+
+instance impl_range_index_array t len n : t_Index (t_Array t len) (t_Range (int_t n)) = 
+  let i = impl_index_range_slice t n in
+  { f_Output = i.f_Output
+  ; in_range = (fun (s: t_Array t len) r -> i.in_range s r)
+  ; f_index = (fun s r -> i.f_index s r) }
+  
+instance impl_range_to_index_array t len n : t_Index (t_Array t len) (t_RangeTo (int_t n)) = 
+  let i = impl_index_range_to_slice t n in
+  { f_Output = i.f_Output
+  ; in_range = (fun (s: t_Array t len) r -> i.in_range s r)
+  ; f_index = (fun s r -> i.f_index s r) }
+
+instance impl_range_from_index_array t len n : t_Index (t_Array t len) (t_RangeFrom (int_t n)) = 
+  let i = impl_index_range_from_slice t n in
+  { f_Output = i.f_Output
+  ; in_range = (fun (s: t_Array t len) r -> i.in_range s r)
+  ; f_index = (fun s r -> i.f_index s r) }
 
 open Rust_primitives.Hax
 
 let update_at_tc_array_range_super t l n: t_Index (t_Array t l) (t_Range (int_t n))
   = FStar.Tactics.Typeclasses.solve
+let update_at_tc_array_range_to_super t l n: t_Index (t_Array t l) (t_RangeTo (int_t n))
+  = FStar.Tactics.Typeclasses.solve
+let update_at_tc_array_range_from_super t l n: t_Index (t_Array t l) (t_RangeFrom (int_t n))
+  = FStar.Tactics.Typeclasses.solve
 
 val update_at_array_range t l n
   (s: t_Array t l) (i: t_Range (int_t n) {(update_at_tc_array_range_super t l n).in_range s i})
   : (update_at_tc_array_range_super t l n).f_Output -> t_Array t l
-  
-instance update_at_tc_array t l n: update_at_tc (t_Array t l) (t_Range (int_t n)) = {
+val update_at_array_range_to t l n
+  (s: t_Array t l) (i: t_RangeTo (int_t n) {(update_at_tc_array_range_to_super t l n).in_range s i})
+  : (update_at_tc_array_range_to_super t l n).f_Output -> t_Array t l
+val update_at_array_range_from t l n
+  (s: t_Array t l) (i: t_RangeFrom (int_t n) {(update_at_tc_array_range_from_super t l n).in_range s i})
+  : (update_at_tc_array_range_from_super t l n).f_Output -> t_Array t l
+
+instance update_at_tc_array_range t l n: update_at_tc (t_Array t l) (t_Range (int_t n)) = {
   super_index = update_at_tc_array_range_super t l n;
   update_at = update_at_array_range t l n
+}
+instance update_at_tc_array_range_to t l n: update_at_tc (t_Array t l) (t_RangeTo (int_t n)) = {
+  super_index = update_at_tc_array_range_to_super t l n;
+  update_at = update_at_array_range_to t l n
+}
+instance update_at_tc_array_range_from t l n: update_at_tc (t_Array t l) (t_RangeFrom (int_t n)) = {
+  super_index = update_at_tc_array_range_from_super t l n;
+  update_at = update_at_array_range_from t l n
 }
