proof-libs/fstar/core/Core.Array.fst
@@ -5,3 +5,6 @@ type t_TryFromSliceError = | TryFromSliceError
 
 let impl_23__map n (arr: t_Array 'a n) (f: 'a -> 'b): t_Array 'b n 
   = map_array arr f
+
+let impl_23__as_slice len (arr: t_Array 'a len): t_Slice 'a = arr
+
